Versão da noite

LeanProjeto2/StarLang.lean
@@ -1,4 +1,10 @@
+-- -------------------------------------------------------------
+--            Star Language (atualizada)
+-- -------------------------------------------------------------
+
+-- We import the definitions from the first-order language L:
 import LeanProjeto2.FOL
+import MathLib.Tactic
 
 namespace StarLang
 
@@ -15,11 +21,11 @@ def G := ground                         -- notation G => ground
 notation t "⟶" t1 => arrow t t1
 notation t "⋆" => star t
 
--- --------------------------
--- TERMS E CONSTANTS (p.9-12)
--- --------------------------
+-- ----------------------------
+-- TERMS and CONSTANTS (p.9-12)
+-- ----------------------------
 
-def Sym : Type := String deriving BEq, DecidableEq, Repr
+-- def Sym : Type := String deriving BEq, DecidableEq, Repr
 
 -- DEFINITION 1.2 (p.8-9): Terms of L^{omega}_*
 inductive Term --where
@@ -29,16 +35,9 @@ inductive Term --where
 | sing                                  -- star constants:  𝔰
 | bUnion                                --                  ∪ (binary union)
 | iUnion                                --                  ∪ (indexed union)
-| var : string → Term                   -- variables
+| var : String → Term                   -- variables
 | app : Term → Term → Term              -- application of terms
---deriving BEq, DecidableEq, Repr
-
---namespace Term
--- Notation for Terms
---infixl:70 " □ " => app
---prefix:90 "` " => var
-
--- (x:string) (var x)
+--deriving Repr                                                                     -- DÁ ERRO
 
 -- NOTATION: Notation for combinators and star constants
 notation "Π₁" => Term.pi
@@ -47,514 +46,305 @@ notation "𝔰₁" => Term.sing
 notation "∪₁" => Term.bUnion
 notation "ind_⋃₁" => Term.iUnion
 notation t₁ "·" t₂ => Term.app t₁ t₂
---notation "⁅"t₁ t₂"⁆" => Term.app t₁ t₂
 
 open Term
 
-/-
--- Substitution function for Terms
-def subst : Term → Sym → Term → Term
-| (var x), y, v => if x = y then v else var x
-| pi, _, _ => pi
-| sigma, _, _ => sigma
-| sing, _, _ => sing
-| bUnion, _, _ => bUnion
-| iUnion, _, _ => iUnion
-| (app l m), y, v => app (subst l y v) (subst m y v)
--/
+-- ------------------------------------------------------
+-- TYPECHECKING THE TERMS OF L^{omega}_*
+-- We typecheck the components of the formulas of L^ω_*.
+-- This guarantees that the formulas have admissible types.
+-- ------------------------------------------------------
 
+inductive Term_TypeChecking : Term → FType → Prop
+| tcLcons (t : LTerm) : Term_TypeChecking (lcons t) G                                                           -- L-constants have type G
+| tcPi {σ τ} : Term_TypeChecking pi (σ ⟶ (τ ⟶ σ))                                                             -- Π_{σ,τ} : σ ⟶ (τ ⟶ σ)
+| tcSigma {σ τ ρ}: Term_TypeChecking sigma ((σ ⟶ (τ ⟶ ρ)) ⟶ ((σ ⟶ τ) ⟶ (σ ⟶ ρ)))                           -- Σ_{σ,τ,ρ} : (σ ⟶ (τ ⟶ ρ)) ⟶ ((σ ⟶ τ) ⟶ (σ ⟶ ρ))
+| tcSing {σ}: Term_TypeChecking sing (σ ⟶ σ⋆)                                                                  -- 𝔰_{σ} : σ⋆
+| tcBUnion {σ}: Term_TypeChecking bUnion (σ⋆ ⟶ (σ⋆ ⟶ σ⋆))                                                      -- ∪_{σ} : σ⋆ ⟶ (σ⋆ ⟶ σ⋆)
+| tcIUnion {σ τ} : Term_TypeChecking iUnion (σ⋆ ⟶ ((σ ⟶ τ⋆) ⟶ τ⋆))                                            -- ∪_{σ} : σ⋆ ⟶ ((σ ⟶ τ⋆) ⟶ τ⋆)
+| tcVar {x σ}: Term_TypeChecking (var x) σ                                                                       -- Variables x : σ
+| tcApp {t₁ t₂ σ τ}: Term_TypeChecking t₁ (σ ⟶ τ) → Term_TypeChecking t₂ σ → Term_TypeChecking (app t₁ t₂) τ    -- If t₁ : (σ ⟶ τ) and t₂ : σ, then t₁t₂ : τ
 
--- Typing the terms of L^{omega}_*   (term type checking)
-inductive TypeChecking : Term → FType → Prop
-| tcLcons (t : LTerm) : TypeChecking (lcons t) G                                                  -- L-constants have type G
-| tcPi {σ τ} : TypeChecking pi (σ ⟶ (τ ⟶ σ))                                                    -- Π_{σ,τ} : σ ⟶ (τ ⟶ σ)
-| tcSigma {σ τ ρ}: TypeChecking sigma ((σ ⟶ (τ ⟶ ρ)) ⟶ ((σ ⟶ τ) ⟶ (σ ⟶ ρ)))                  -- Σ_{σ,τ,ρ} : (σ ⟶ (τ ⟶ ρ)) ⟶ ((σ ⟶ τ) ⟶ (σ ⟶ ρ))
-| tcSing {σ}: TypeChecking sing (σ ⟶ σ⋆)                                                         -- 𝔰_{σ} : σ⋆
-| tcBUnion {σ}: TypeChecking bUnion (σ⋆ ⟶ (σ⋆ ⟶ σ⋆))                                            -- ∪_{σ} : σ⋆ ⟶ (σ⋆ ⟶ σ⋆)
-| tcIUnion {σ τ} : TypeChecking iUnion (σ⋆ ⟶ ((σ ⟶ τ⋆) ⟶ τ⋆))                                   -- ∪_{σ} : σ⋆ ⟶ ((σ ⟶ τ⋆) ⟶ τ⋆)
-| tcVar {x σ}: TypeChecking (var x) σ                                                             -- Variables x : σ
-| tcApp {t₁ t₂ σ τ}: TypeChecking t₁ (σ ⟶ τ) → TypeChecking t₂ σ → TypeChecking (app t₁ t₂) τ    -- If t₁ : (σ ⟶ τ) and t₂ : σ, then t₁t₂ : τ
-
-open TypeChecking
+open Term_TypeChecking
 
 
 -- ------------------
 -- FORMULAS (p.12-14)
 -- ------------------
 
--- DEFINITION 1.6 (p.11): Atomic formulas of L^{omega}_*
-inductive AtomicFormula
-| lForm : LFormula → AtomicFormula                                  -- Remark 1.9: The atomic formulas of L^{omega}_* include the atomic formulas of L
-| rel : string → List Term → AtomicFormula                          -- R(t₁, ..., tₙ) with R relational symbol of L and t₁,...,tₙ ground terms in L^{omega}_*
-| eq : FType → Term → Term → AtomicFormula                          -- t =σ q
-| mem : FType → Term → Term → AtomicFormula                         -- t ∈σ q
+/-
+We define the formulas of L^ω_*:
+  a) The atomic formulas (definition 1.6 - p.11)
+  b) The base formulas (definition 1.10 - p.14)
+  c) The formulas (definition 1.7 - p.13)
+-/
 
--- Typing the components of the atomic formulas of L^{omega}_* (atomic formulas type checking)
-inductive AtomicTypeChecking : AtomicFormula → Prop
-| tcRel {R l_terms} :                             -- R é relational symbol DE L (falta); l_terms é uma lista de termos
-    (∀ t, t ∈ l_terms → TypeChecking t G) →
-    AtomicTypeChecking (AtomicFormula.rel R l_terms)
-| tcEq {σ t₁ t₂} :
-    TypeChecking t₁ σ →
-    TypeChecking t₂ σ →
-    AtomicTypeChecking (AtomicFormula.eq σ t₁ t₂)
-| tcMem {σ t₁ t₂} :
-    TypeChecking t₁ σ →
-    TypeChecking t₂ (σ⋆) →
-    AtomicTypeChecking (AtomicFormula.mem σ t₁ t₂)
-
--- NOTATION: Notation for the equality and the membership symbols
---notation t₁ "=_" t₂ => AtomicFormula.eq t₁ t₂
---notation t₁ "∈_"σ t₂ => AtomicFormula.mem σ t₁ t₂
-
-open AtomicFormula
-
--- DEFINITION 1.10 (p.14): Base formulas of L^{omega}_*
-inductive BaseFormula
-| batom : AtomicFormula → BaseFormula                                   -- Atomic formulas are base formulas
-| bnot : BaseFormula → BaseFormula                                      -- If A is a base formula, then so is (¬A)
-| bor : BaseFormula → BaseFormula → BaseFormula                         -- If A and B are base formulas, then so is (A∨B)
-| bboundedForall : string → FType → Term → BaseFormula → BaseFormula    -- If A is a base formula, then so is (∀x∈t A)
-
---#check (A : AtomicFormula) batom A
-def SomeFormula (A : AtomicFormula) : BaseFormula := BaseFormula.batom A        -- TESTE
-#check SomeFormula                                                              -- TESTE
-
--- DEFINITION 1.7 (p.13): Formulas of L^{omega}_*
 inductive Formula
-| Fbase : BaseFormula → Formula                                         -- Base formulas are formulas
-| Fnot : Formula → Formula                                              -- If A is a formula, then so is (¬A)
-| For : Formula → Formula → Formula                                     -- If A and B are formulas, then so is (A∨B)
-| FboundedForall : string → FType → Term → Formula → Formula            -- If A is a formula, then so is (∀x∈t A)
-| FunboundedForall : string → FType → Formula → Formula                 -- If A is a base formula, then so is (∀x A)
+| L_Form : LFormula → Formula
+| rel : string → List Term → Formula                                -- R(t₁, ..., tₙ) with R relational symbol of L and t₁,...,tₙ ground terms in L^{omega}_*
+| eq : Term → Term → Formula                                        -- t =σ q
+| mem : Term → Term → Formula                                       -- t ∈σ q
+| not : Formula → Formula                                           -- If A is a formula, then so is (¬A)
+| or : Formula → Formula → Formula                                  -- If A and B are formulas, then so is (A∨B)
+| unbForall : string → Formula → Formula                            -- If A is a base formula, then so is (∀x A)
+| bForall : string → Term → Formula → Formula                       -- If A is a formula, then so is (∀x∈t A)
 
--- Type checking for base formulas
-inductive BaseFormulaTypeChecking : BaseFormula → Prop
-| tcBatom {A} :
-    AtomicTypeChecking A → BaseFormulaTypeChecking (BaseFormula.batom A)
-| tcBnot {A} :
-    BaseFormulaTypeChecking A → BaseFormulaTypeChecking (BaseFormula.bnot A)
-| tcBor {A B} :
-    BaseFormulaTypeChecking A →
-    BaseFormulaTypeChecking B →
-    BaseFormulaTypeChecking (BaseFormula.bor A B)
-| tcBboundedForall {x σ t A} :
-    TypeChecking (Term.var x) σ →
-    TypeChecking t (σ⋆) →
-    BaseFormulaTypeChecking A →
-    BaseFormulaTypeChecking (BaseFormula.bboundedForall x σ t A)
 
--- Type checking for formulas
-inductive FormulaTypeChecking : Formula → Prop
-| tcFbase {A} :
-    BaseFormulaTypeChecking A → FormulaTypeChecking (Formula.Fbase A)
-| tcFnot {A} :
-    FormulaTypeChecking A → FormulaTypeChecking (Formula.Fnot A)
-| tcFor {A B} :
-    FormulaTypeChecking A →
-    FormulaTypeChecking B →
-    FormulaTypeChecking (Formula.For A B)
-| tcFboundedForall {x σ t A} :
-    TypeChecking (Term.var x) σ →
-    TypeChecking t (σ⋆) →
-    FormulaTypeChecking A →
-    FormulaTypeChecking (Formula.FboundedForall x σ t A)
-| tcFunboundedForall {x σ A} :
-    TypeChecking (Term.var x) σ →
-    FormulaTypeChecking A →
-    FormulaTypeChecking (Formula.FunboundedForall x σ A)
-
-open BaseFormula
 open Formula
 
-def AB (A B : Formula) : Formula := Formula.For A B             -- TESTE
-def AB2 (A B : Formula) : Formula := For A B                    -- TESTE
-def ABC (A B C : Formula) : Formula := For A (For B C)          -- TESTE
+-- NOTATION: Notation for the equality and the membership symbols
+notation t₁ "=₁" t₂ => Formula.eq t₁ t₂
+notation t₁ "∈₁" t₂ => Formula.mem t₁ t₂
 
 -- NOTATION: Notation for the primitive symbols ¬, ∨, ∀x and ∀x∈t in L^{omega}_*
-notation "¬₁" A => Fnot A
-notation A "∨₁" B => For A B
-notation "b∀₁" x σ t A => FboundedForall x σ t A
-notation "V₁" x σ A => FunboundedForall x σ A
+notation "¬₁" A => not A
+notation A "∨₁" B => or A B
+notation "V₁" => unbForall
+notation "bV₁" => bForall
+-- notation "b∀₁" x t A => bForall x t A
 
-def ABC2 (A B C : Formula) : Formula := A ∨₁ (B ∨₁ C)           -- TESTE
-def ABC3 (A B C : Formula) : Formula := (A ∨₁ B) ∨₁ C           -- TESTE
-#check ABC2                                                     -- TESTE
---def ABCABC2 (A B C : Formula) : Formula → Formula := (ABC2 A B C) → (ABC3 A B C)
---def ABCABC (A B C : Formula) : Formula → Formula := A ∨₁ (B ∨₁ C) → (A ∨₁ B) ∨₁ C
+-- DEFINITION 1.8 (p.14): The bounded existential quantifier ∃x∈t (defined symbol)
+
+-- The unbounded existential quantifier ∃x A
+def E₁ (x : string) (A : Formula) : Formula :=
+  ¬₁(unbForall x (¬₁ A))
+
+-- The bounded existential quantifier ∃x A
+def bE₁ (x : string) (t : Term) (A : Formula) : Formula :=
+  ¬₁(bForall x t (¬₁ A))
+
+-- Testing the notation
+-- def Notation_test (x : string) (t : Term) (A : Formula) : Formula := bV₁ x t A
+-- #check Notation_test
 
 -- --------------------
--- DEFINED SYMBOLS: Usual logical abbreviations for the defined symbols ∧, →, ↔, ∃x and ∃x∈t in L^{omega}_* (p.8 and p.14)
+-- DEFINED SYMBOLS (p.8 and p.14):
+-- Usual logical abbreviations for the defined symbols ∧, →, ↔, ∃x and ∃x∈t in L^{omega}_*
 -- --------------------
 
 -- Conjunction:  A ∧ B := ¬(¬A∨¬B)
 @[simp]
-def Fand (A B : Formula) : Formula :=
+def F_and (A B : Formula) : Formula :=
   ¬₁ ((¬₁ A) ∨₁ (¬₁ B))
--- have (¬₁ ((¬₁ A) ∨₁ (¬₁ B))) by
+
+notation A "∧₁" B => F_and A B
 
 -- Implication:  A → B := ¬ A ∨ B
 @[simp]
-def Fimplies (A B : Formula) : Formula :=
+def F_implies (A B : Formula) : Formula :=
   (¬₁ A) ∨₁ B
 
-notation A "∧₁" B => Fand A B
-notation A "→₁" B => Fimplies A B
+notation A "→₁" B => F_implies A B
 
 -- Equivalence:  A ↔ B := (A → B) ∧ (B → A)
 @[simp]
-def Fiff (A B : Formula) : Formula :=
-  (A →₁ B) ∧₁ (B →₁ A)
+def F_iff (A B : Formula) : Formula :=
+  ¬₁ ((¬₁((¬₁A) ∨₁ B)) ∨₁ (¬₁((¬₁B) ∨₁ A)))
+  -- (A →₁ B) ∧₁ (B →₁ A)
+  -- (¬₁ A ∨₁ B) ∧₁ (¬₁ B ∨₁ A)
 
--- Existential quantification:  ∃x A := ¬ (∀x (¬ A))
---def Fexists (x : string) (σ : FType) (A : Formula) : Formula :=
---  ¬₁(∀₁ "x" σ (¬₁A))
+notation A "↔₁" B => F_iff A B
 
-notation A "↔₁" B => Fiff A B
--- notation "∃₀" x A => exists_L x A
+-- ------------------------------------------------------
+-- CHECKING FORMULAS:
+-- ------------------------------------------------------
 
--- ∃x A := ¬ (∀x (¬ A))                                 -- TESTE
---def lexists (x : LVar) (A : LFormula) : LFormula :=   -- TESTE
---  ¬₁ (∀₁ x (¬₁ A))                                    -- TESTE
+-- Checks whether a given formula is atomic:
+inductive isAtomic : Formula → Prop
+| at_rel : isAtomic (rel x l_term)
+| at_eq : isAtomic (eq t₁ t₂)
+| at_mem : isAtomic (mem t₁ t₂)
 
-def teste3 (A : Formula) := ¬₁(¬₁ A)                    -- TESTE
-#check teste3                                           -- TESTE
+-- Checks whether a given formula is base:
+inductive isBase : Formula → Prop
+| b_atom : isAtomic A → isBase A                                                -- Atomic formulas are base formulas
+| b_not (h: isBase A) : isBase (not A)                                          -- If A is base, then so is ¬₁A
+| b_or (h1: isBase A) (h2 : isBase B) : isBase (or A B)                         -- If A and B are base, then so is A∨₁B
+| b_bForall (x : string) (t : Term) (h : isBase A) : isBase (bForall x t A)     -- If A is base, then so is ∀x∈t A
+
+open isBase
+
+-- Example: Let A be an atomic formula (assumption h), then it is base.
+example (A : Formula) (h : isAtomic A)  : (isBase A) := by
+  exact b_atom h
+
+example (A B : Formula) (hA_at : isAtomic A) (hB_b : isBase B) : (isBase (A∨₁B)) := by
+  have h := b_atom hA_at
+  exact b_or h hB_b
+
+-- ------------------------------------------------------
+-- LEMMAS: Defined symbols of base formulas are also base
+-- ------------------------------------------------------
+
+-- Lemma Conj_base states that if A and B are base formulas, then so is their conjunction A ∧ B
+lemma Conj_base (A B : Formula) (hA : isBase A) (hB : isBase B) : (isBase (A∧₁B)) := by
+  unfold F_and
+  have h_nA := b_not hA
+  have h_nB := b_not hB
+  have h_or_nAnB := b_or h_nA h_nB
+  exact b_not h_or_nAnB
+
+-- Lemma Imp_base states that if A and B are base formulas, then so is their implication A → B
+lemma Imp_base (A B : Formula) (hA : isBase A) (hB : isBase B) : (isBase (A→₁B)) := by
+  unfold F_implies
+  have h_nA := b_not hA
+  exact b_or h_nA hB
+
+-- Lemma Iff_base states that if A and B are base formulas, then so is their equivalence A ↔ B
+lemma Iff_base (A B : Formula) (hA : isBase A) (hB : isBase B) : (isBase (A↔₁B)) := by
+  unfold F_iff
+  have h_nA := b_not hA
+  have h_nB := b_not hB
+  have h_or_nAB := b_or h_nA hB
+  have h_or_nBA := b_or h_nB hA
+  have h_n_or_nAB := b_not h_or_nAB
+  have h_n_or_nBA := b_not h_or_nBA
+  have H := b_or h_n_or_nAB h_n_or_nBA
+  exact b_not H
+
+-- Lemma unbForall_base states that if A is a base formula, then so is ∀x∈t A
+lemma unbForall_base (A : Formula) (x : string) (t : Term) (hA : isBase A) : (isBase (bE₁ x t A)) := by
+  unfold bE₁
+  have h_nA := b_not hA
+  have h_unbForall_nA := b_bForall x t h_nA
+  exact b_not h_unbForall_nA
+
+-- ------------------------------------------------------
+-- TYPECHECKING
+-- We typecheck the components of the formulas of L^ω_*.
+-- This guarantees that the formulas have admissible types.
+-- ------------------------------------------------------
+
+inductive Formula_TypeChecking : Formula → Prop
+| tcRel {R l_terms} :                                               -- R é relational symbol DE L (falta); l_terms é uma lista de termos
+    (∀ t, t ∈ l_terms → Term_TypeChecking t G) →
+    Formula_TypeChecking (Formula.rel R l_terms)
+| tcEq {σ t₁ t₂} :
+    Term_TypeChecking t₁ σ →
+    Term_TypeChecking t₂ σ →
+    Formula_TypeChecking (Formula.eq t₁ t₂)
+| tcMem {σ t₁ t₂} :
+    Term_TypeChecking t₁ σ →
+    Term_TypeChecking t₂ (σ⋆) →
+    Formula_TypeChecking (Formula.mem t₁ t₂)
+| tcNot {A} :
+    Formula_TypeChecking A → Formula_TypeChecking (Formula.not A)
+| tcOr {A B} :
+    Formula_TypeChecking A →
+    Formula_TypeChecking B →
+    Formula_TypeChecking (Formula.or A B)
+| tcbForall {x σ t A} :
+    Term_TypeChecking (Term.var x) σ →
+    Term_TypeChecking t (σ⋆) →
+    Formula_TypeChecking A →
+    Formula_TypeChecking (Formula.bForall x t A)
+| tcunbForall {x σ A} :
+    Term_TypeChecking (Term.var x) σ →
+    Formula_TypeChecking A →
+    Formula_TypeChecking (Formula.unbForall x A)
+
 
 -- --------------------------------------
--- Notation for the bounded and unbounded universal quantifier
-
-def V (x : string) (σ : FType) (A : Formula) : Formula := FunboundedForall x σ A
-def bV (x : string) (σ : FType) (t : Term) (A : Formula) : Formula := FboundedForall x σ t A
-
--- --------------------------------------
-
--- DEFINITION 1.8 (p.14): The bounded existential quantifier ∃x∈t (defined symbol)
-
--- F_unb_exists
-def E (x : string) (σ : FType) (A : Formula) : Formula :=
-  ¬₁(FunboundedForall x σ (¬₁ A))
-
--- F_b_exists
-def bE (x : string) (σ : FType) (t : Term) (A : Formula) : Formula :=
-  ¬₁(FboundedForall x σ t (¬₁ A))
-
--- --------------------
--- Acrescentar algo que checks whether a formula is base or not
---  + acrescentar que simbolos definidos também deixam as base formulas closed
--- --------------------
-
--- CHECK SE É BASE
-
-def isBase : Formula → Bool
-| Fbase _ => true
-| _ => false
-
-#check isBase
-
---@[simp]
-def isBaseFormula : Formula → Bool
-| Fbase _ => true
-| ¬₁ (Fbase _) => true
-| (Fbase _) ∨₁ (Fbase _) => true
-| FboundedForall _ _ _ (Formula.Fbase _) => true
-| _ => false
-
--- Ex1.4(1). tx : τ where t : σ → τ and x : σ                                 -- TESTE
-example (σ τ : FType) (t : Term) (x : string)                                 -- TESTE
-    (h1: TypeChecking t (σ ⟶ τ))                                             -- TESTE
-    (h2 : TypeChecking (var x) σ) : TypeChecking (app t (var x)) τ :=         -- TESTE
-  by                                                                          -- TESTE
-   exact TypeChecking.tcApp h1 h2                                             -- TESTE
-
-lemma teste1 (A : BaseFormula)                                                -- TESTE
-  (hA : isBaseFormula (Fbase A))                                              -- TESTE
-  (hB : isBaseFormula (Fbase B)) : isBaseFormula ((Fbase A) ∨₁ (Fbase B)) :=  -- TESTE
-  by                                                                          -- TESTE
-    simp [isBaseFormula]                                                      -- TESTE
-
-#check teste1                                                                 -- TESTE
-
-
-
--- Lemma: ¬₁ ((¬₁ A) ∨₁ (¬₁ B)) is a base formula
---AQUIlemma neg_disjunction_is_base_formula (A B : BaseFormula) (h: bnot (bor (bnot A) (bnot B))) : BaseFormula := sorry
---begin
---  exact BaseFormula.bnot (BaseFormula.bor (BaseFormula.bnot A) (BaseFormula.bnot B)),
---end
-
---example (A : BaseFormula) (hA : isBaseFormula (Fbase A)) (hB : isBaseFormula (Fbase B)) : isBaseFormula ((¬₁ (Fbase A)) ∨₁ (Fbase B)) :=
---  by
---    simp [isBaseFormula]
-  -- by
-  -- exact isBaseFormula
-
--- lemma (A B : FBase): (A ∧₁ B) : FBase :=
--- Lemma: if A and B are BaseFormula, then A ∧₁ B is a BaseFormula
---lemma and_is_baseformula (A B : BaseFormula) : isBaseFormula ((Fbase A) ∧₁ (Fbase B)) = true := sorry
-  ----by
-    -- Acho que devia simplificar usando Fand
-    -----simp
-    -----have h1 := isBaseFormula ((Fbase A) ∨₁ (Fbase B))
-  --by unfold Fand (Fbase A) (Fbase B)
-  --by unfold Fand ; simp [isBaseFormula]
-
-
-
-
--- ----------------------------------------
--- EXAMPLE 1.6 (p.14): Base formulas or not
--- ----------------------------------------
-
--- example (A : Formula) (B : FBase) (σ τ : FTypes)
-
-
-
-
-
-
--- --------------------
 -- AXIOMS
--- --------------------
-
--- SHOENFIELD'S CALCULUS (Axiom 1.1)
-
--- -----------------------------------------------------------------------------------
--- -------------------------- AXIOM SCHEMA -------------------------------------------
--- -----------------------------------------------------------------------------------
-
--- Axiom schema:
-
--- --------------------------- Excluded middle ---------------------------------------
--- Excluded middle
-
--- axiom ExcMid (A : Formula) : (¬₁ A) ∨₁ A
--- axiom ExcMid (A : Formula) : For (Fnot A) A
-
-
--- Excluded middle DEFINITION
-def excluded_middle_axiom (A : Formula) : Formula :=
-  (¬₁ A) ∨₁ A
---  For (Fnot A) A
-
--- Excluded middle AXIOM + AXIOM INSTANCE
-axiom excluded_mid_axiom (A : Formula) : Formula
-axiom excluded_mid_instance (A : Formula) : excluded_middle_axiom A = (¬₁ A) ∨₁ A
-
--- --------------------------- Substitution (TBDone)---------------------------------
--- Substituion
-
--- -----------------------------------------------------------------------------------
--- --------------------------- RULES -------------------------------------------------
--- -----------------------------------------------------------------------------------
-
--- Rules:
-
--- --------------------------- Expansion ---------------------------------------------
--- Expansion
-
-def expansion_r (A B : Formula) : Formula :=
-  B ∨₁ A
-
-axiom expansion_rule (A B : Formula) : Formula
-axiom expansion_instance (A B : Formula) : expansion_rule A B = B ∨₁ A
-
--- --------------------------- Contraction ------------------------------------------
--- Contraction
-
-def contraction_r (A : Formula) : Formula :=
-  A ∨₁ A
-
-axiom contraction_rule (A : Formula) : Formula
-axiom contraction_instance (A : Formula) : contraction_rule A = A ∨₁ A
-
--- --------------------------- Associativity ----------------------------------------
--- Associativity
-
--- axiom associativity {A B C : Formula} : (A ∨₁ (B ∨₁ C)) → (A ∨₁ B) ∨₁ C
-
-
---def associativity_r (A B C : Formula) (h : A ∨₁ (B ∨₁ C)) : Formula :=
---   (A ∨₁ B) ∨₁ C
-
---def associativity_r (A B C : Formula) (h : (For A (For B C))) : Formula :=
---   For (For A B) C
-
---def associativity_r (A B : Formula) : Formula → Formula :=
---  A → A
-
---axiom associativity_rule (A B C : Formula) : Formula
---axiom ass_inst (A B C : Formula) : associativity_rule A B C = (A∨₁(B∨₁C) → (A∨₁B)∨₁C)
---axiom associativity_instance (A B C : Formula) : (associativity_rule A B C) = A ∨₁ (B ∨₁ C) → (A ∨₁ B) ∨₁ C
-
---axiom associativity (A B C : Formula) : ((A ∨₁ B) ∨₁ C) → (A ∨₁ (B ∨₁ C))
-
--- --------------------------- Cut --------------------------------------------------
--- Cut
-
--- --------------------------- ∀-introduction ---------------------------------------
--- ∀-introduction
-
-
-
-
--- -----------------------------------------------------------------------------------
--- --------------------------- OTHER AXIOMS -------------------------------------------------
--- -----------------------------------------------------------------------------------
-
-
--- EQUALITY AXIOMS (Axiom 1.2)
-
---axiom equality_reflexivity (σ : FType) (x : var) : Formula :=
---  ∀₀ x (Term.var x =_σ Term.var x)
-
-
--- PROPOSITION 1.1: Symmetry and transitivity of equality (higher types)
-
--- Symmetry of equality   WRONG -> precisamos de TypeChecking?
---theorem symmetry_of_eq (σ : FType) (x y : string): eq σ (var x) (var y) → eq σ (var y) (var x) := sorry
--- by intro a intro b exact tcEq hx hy
--- λ h, h.symm
-
--- Types in the symmetry of equality   WRONG -> precisamos de TypeChecking?
---theorem symmetry_of_eq (σ : FType) (x y : string)
---    (hx : TypeChecking (var x) σ)
---    (hy : TypeChecking (var y) σ) : (var x) "=_"σ (var y) → (var y) "=_"σ (var x) := sorry
--- by intro a intro b exact tcEq hx hy
--- λ h, h.symm
-
--- #check AtomicFormula.eq σ (var x) (var y)
-
--- Types in the symmetry of equality   WRONG -> precisamos de TypeChecking?
---theorem symmetry_of_eq2 (σ : FType) (x y : string)
---    (hx : TypeChecking (var x) σ)
---    (hy : TypeChecking (var y) σ)
---    (hy : TypeChecking (var y) σ): AtomicFormula.eq σ (var x) (var y) → AtomicFormula.eq σ (var y) (var x) := sorry
--- by intro a intro b exact tcEq hx hy
--- λ h, h.symm
-
--- notation t₁ "=_"σ t₂ => AtomicFormula.eq σ t₁ t₂
-
--- Transitivity of equality   WRONG -> precisamos de TypeChecking?
--- theorem transitivity_of_eq (σ : FType) (x y z : string) (hx : TypeChecking.tcVar x σ) (hy : TypeChecking.tcVar y σ) (hz : TypeChecking.tcVar z σ) : (var x) "=_"σ (var y) → (var y) "=_"σ (var z) → (var x) "=_"σ (var z) :=
--- λ hxy hyz, hxy.trans hyz
-
-
-lemma example_lemma (P Q : Prop) (h : P → Q) (p : P) : Q :=
-  h p
-
--- notation t₁ "=_" t₂ σ => AtomicFormula.eq t₁ t₂ σ
-
---lemma example_lemma2 (t₁ t₂ : Term) (σ : FType) : (AtomicFormula.eq t₁ t₂ σ) → (AtomicFormula.eq t₁ t₂ σ) := sorry
-
--- inductive AtomicFormula2
--- | atrel : string → List Term → AtomicFormula2  -- R(t₁, ..., tₙ)
--- | ateq : Term → Term → FType → AtomicFormula2  -- t =σ q
--- | atmem : FType → Term → Term → AtomicFormula2 -- t ∈σ q
-
--- lemma example_lemma2 (t₁ t₂ : Term) (σ : FType) (h: t₁ "=_" t₂ σ) : (t₁ "=_" t₂ σ) := sorry
---  intro h
---  exact h
-
--- ----------------------------------------------------------------------------------------------------------
--- ----------------------------------------------------------------------------------------------------------
-
--- -----------------AXIOM FOR THE BOUNDED UNIVERSAL QUANTIFIER (Axiom 1.3) -----------------
-
-def AxU (σ : FType) (x t : Term) (A : Formula) : Formula            -- FALTA A(x)
-  := (bV x σ t A) ↔₁ (V x σ ((Fbase (batom (mem σ x t))) →₁ A))
-
--- ----------------------------- COMBINATOR AXIOMS (Axiom 1.4) -----------------------------
-
-def AxC₁ (σ : FType) (p q : Term) : AtomicFormula       -- FALTA TYPECHECKING -> TBDONE AS LEMMA
-  := eq σ ((Π₁·p)·q) q
-
--- (h: typechecks pri,eirq tqu qnd  )
-def AxC₂ (τ : FType) (p q t : Term) : AtomicFormula     -- FALTA TYPECHECKING
-  := eq τ (((Σ₁·p)·q)·t) ((p·t)·(q·t))
-
-
--- ---------------- PRIMARY AXIOMS FOR THE STAR CONSTANTS (Axiom 1.5) ----------------------
-
-def AxP₁ (τ : FType) (x y : Term) : AtomicFormula
-  := eq (τ⋆) ((ind_⋃₁·(𝔰₁·x))·y) (x·y)
-
-def AxP₂_atom (τ : FType) (x y z : Term) : AtomicFormula
-  := eq (τ⋆) ((ind_⋃₁·((∪₁·x)·y))·z) ((∪₁·((ind_⋃₁·x)·z))·((ind_⋃₁·y)·z))
-
-def AxP₂_base (τ : FType) (x y z : Term) : BaseFormula
-  := batom (eq (τ⋆) ((ind_⋃₁·((∪₁·x)·y))·z) ((∪₁·((ind_⋃₁·x)·z))·((ind_⋃₁·y)·z)))
-
-def AxP₂_formula (τ : FType) (x y z : Term) : Formula
-  := Fbase (batom (eq (τ⋆) ((ind_⋃₁·((∪₁·x)·y))·z) ((∪₁·((ind_⋃₁·x)·z))·((ind_⋃₁·y)·z))))
-
--- -------------- SECONDARY AXIOMS FOR THE STAR CONSTANTS (Axiom 1.6) ----------------------
-
-def AxS₁ (σ : FType) (x y : Term) : Formula
-  := Fbase (batom (mem σ x (𝔰₁·y))) ↔₁ Fbase (batom (eq σ x y))
-
---def AxS₁_ab (σ : FType) (x y : Term) : Formula                  -- ABBREVIATION NOT WORKING
---  := Fbase (batom (x ∈_ σ (𝔰₁·y))) ↔₁ Fbase (batom (x ∈_ σ y))
-
-def AxS₂ (σ : FType) (x a b: Term) : Formula
-  := Fbase (batom ( mem σ x ((∪₁·a)·b) )) ↔₁  ( ( Fbase ((batom (mem σ x a))) ∨₁ Fbase ((batom (mem σ x b)) )))
-
-def AxS₃ (σ : FType) (x a b f : Term) : Formula
-  := (Fbase (batom (mem σ b ((ind_⋃₁·a)·f)))) ↔₁ (bE x σ a (Fbase (batom ((mem σ b (f·x))))))
-
--- ---------------------- BOUNDED AXIOM OF CHOICE (Axiom 1.7) -----------------------------
-
--- This está meh!! f não tem de ser variável...
-def bAC  (x y f : string) (σ : FType) (A : Formula) : Formula        -- FALTA: restricted to base formulas | (x y : var) | tirar tipos
-  := (V x σ (E y σ A)) →₁ (E f σ (V x σ (bE y σ ((var f)·(var x)) A)))
-
-
--- SUBSTITUIÇAO
-
--- Pattermatching com "lambda por casos"  FAZER PARA OS OUTROS TERMOS
---@[simp]
---def subst (x : string) (p : Term) : Term → Term
---| (var y) => if x=y then p else var y           -- var substitui logo
---| (app e1 e2) => app (subst x p e1) (subst x p e2)
---| x => x                  -- outra coisa qualquer
-
-
-/-
-
-def subst (x : string) (y : Sym) (v l m : Term) : Term → Sym → Term → Term
-| (var x), y, v => if x = y then v else (var x)
-| pi, _, _ => pi
-| sigma, _, _ => sigma
-| sing, _, _ => sing
-| bUnion, _, _ => bUnion
-| iUnion, _, _ => iUnion
-| (app l m), y, v => app (subst l y v) (subst m y v)
-
--/
-
-
--- CONVERSIONS
-
--- Primeira conversion
-def pi_app_transform : Term → Term
-| (Π₁·q)·_ => q
+-- --------------------------------------
+
+--def normal_form (A B : Formula) (x: string) : Formula → Formula
+--| or A B => A
+--| bForall x A => A
+--| t => t
+
+-- Drei strecher ass gleich, wees net wei dat heescht
+inductive Equivalent : Formula → Formula → Prop
+| id : Equivalent A A
+| comm : Equivalent A B → Equivalent B A
+--| nf_left : Equivalent A B → Equivalent (normal_form A) B
+--| nf_right : Equivalent A B → Equivalent A (normal_form B)
+
+inductive isTrue : Formula → Prop
+| lem : isTrue (A ∨₁ (¬₁A))
+--| substitution : FALTA
+| expansion:
+      isTrue A →
+      ---------------
+      isTrue (A ∨₁ B)
+| contraction :
+      isTrue (A ∨₁ A) →
+      ---------------
+      isTrue A
+| associativity :
+      isTrue (A ∨₁ (B ∨₁ C)) →
+      ---------------
+      isTrue ((A ∨₁ B) ∨₁ C)
+| cut :
+      isTrue (A ∨₁ B) →
+      isTrue ((¬₁A)∨₁C) →
+      ---------------
+      isTrue (B ∨₁ C)
+--| forall_introduction : FALTA
+| equivalence :
+      (Equivalent A B) →
+      isTrue A →
+      isTrue B
+| AxE₁ (x : String) :
+    isTrue ((var x) =₁ (var x))
+--| AxE₂ (x y : String) : isTrue ((((var x) =₁ (var y))∧₁ A) →₁ A)        FALTA: falta A(x) e A(y)
+| AxU (x : String) (t : Term) (A : Formula) :
+    isTrue ((bV₁ x t A) ↔₁ (V₁ x (((var x) ∈₁ t) →₁ A)))
+| AxC₁ (t₁ t₂ : Term) :
+    isTrue (((Π₁·t₁)·t₂) =₁ t₁)
+| AxC₂ (t₁ t₂ t₃ : Term) :
+    isTrue ((((Σ₁·t₁)·t₂)·t₃) =₁ ((t₁·t₃)·(t₂·t₃)))
+| AxP₁ (t₁ t₂ : Term) :
+    isTrue (((ind_⋃₁·(𝔰₁·t₁))·t₂) =₁ (t₂·t₁))
+| AxP₂ (t₁ t₂ t₃ : Term) :
+    isTrue (((ind_⋃₁·((∪₁·t₁)·t₂))·t₃) =₁ ((∪₁·((ind_⋃₁·t₁)·t₃))·((ind_⋃₁·t₂)·t₃)))
+| AxS₁ (t₁ t₂ : Term) :
+    isTrue ((t₁ ∈₁ (𝔰₁·t₂)) ↔₁ (t₁ =₁ t₂))
+| AxS₂ (t₁ t₂ t₃ : Term) : isTrue ((t₁ ∈₁ ((∪₁·t₂)·t₃) ) ↔₁ ((t₁ ∈₁ t₂) ∨₁ (t₁ ∈₁ t₃)))
+| AxS₃ (a f b : Term) : isTrue ((b ∈₁ ((ind_⋃₁·a)·f)) ↔₁ (bE₁ x a (b ∈₁ (f·x))))
+
+-- FALTA: falta o bAC^ω_*
+
+-- TESTE: o lemma eq_symmetry está a dar erro, mas o teste com #check mostra que a sintaxe está good
+def f : Term := var "f"
+def g : Term := var "g"
+
+#check (f =₁ g) →₁ (g =₁ f)
+
+--lemma eq_symmetry : (f =₁ g) →₁ (g =₁ f) := sorry
+
+--theorem tastino (x y : String) : Formula
+
+--lemma eq_symmetry (x y : String) : (((var x) =₁ (var y)) →₁ ((var y) =₁ (var x))) := sorry
+
+--lemma eq_transitivity (x y z : String) : ((((var x) =₁ (var y)) ∧₁ ((var y) =₁ (var z))) →₁ ((var x) =₁ (var z))) := sorry
+
+-- --------------------------------------
+-- COVERSIONS
+-- --------------------------------------
+
+-- Checks whether a term converts to another one
+inductive ConvertsTo : Term → Term → Prop
+| c1_pi {t₁ t₂}: ConvertsTo ((Π₁·t₁)·t₂) t₁
+| c2_sigma {t₁ t₂ t₃}: ConvertsTo (((Σ₁·t₁)·t₂)·t₃) ((t₁·t₃)·(t₂·t₃))
+| c3_indU {t₁ t₂} : ConvertsTo ((ind_⋃₁·(𝔰₁·t₁))·t₂) (t₂·t₁)
+| c4_indU_binU {t₁ t₂ t₃}: ConvertsTo ((ind_⋃₁·((∪₁·t₁)·t₂))·t₃) ((∪₁·((ind_⋃₁·t₁)·t₃))·((ind_⋃₁·t₂)·t₃))
+
+def conv : Term → Term
+| ((Π₁·t₁)·t₂) => t₁
+| ((Σ₁·t₁)·t₂)·t₃ => (t₁·t₃)·(t₂·t₃)
+| (ind_⋃₁·(𝔰₁·t₁))·t₂ => t₂·t₁
+| (ind_⋃₁·((∪₁·t₁)·t₂))·t₃ => (∪₁·((ind_⋃₁·t₁)·t₃))·((ind_⋃₁·t₂)·t₃)
 | t => t
 
--- Example usage
---#eval pi_app_transform p
+def examplinho (q t : Term) := ((Π₁·q)·t)
+--#eval examplinho                                FALTA: falta o REPR que está a dar erro
 
--- Transformation function?
-def pi_app_transform2 : Term → Term
-| (Π₁·q)·_ => q   -- Transforma (Π₁·q)·_ em q
-| t => t             -- Outros casos ficam
+--notation t₁ "▹" t₂ => conv t₁ t₂
 
--- def pi_app_transform2 : Term → Term → Term
--- | p q => q
--- | t => t
+-- FALTA: conversions preserve types
 
-def example_term (q t : Term) : Term := (Π₁·q)·t
-#check example_term
-
-
+-- EXAMPLE 1.10 (p.28)
 
 
 end StarLang
