LeanProjeto2/StarLang_old.lean
@@ -1,0 +1,566 @@
+-- -------------------------------------------------------------
+--            Star Language (desatualizada)
+-- -------------------------------------------------------------
+
+import LeanProjeto2.FOL
+
+namespace StarLang_old
+
+-- Finite types [def 1.1]
+inductive FType : Type
+| ground : FType                        -- G
+| arrow : FType → FType → FType         -- σ → τ
+| star : FType → FType                  -- σ*
+
+open FType
+
+-- Notation for finite types
+def G := ground                         -- notation G => ground
+notation t "⟶" t1 => arrow t t1
+notation t "⋆" => star t
+
+-- --------------------------
+-- TERMS E CONSTANTS (p.9-12)
+-- --------------------------
+
+def Sym : Type := String deriving BEq, DecidableEq, Repr
+
+-- DEFINITION 1.2 (p.8-9): Terms of L^{omega}_*
+inductive Term --where
+| lcons : LTerm → Term                  -- L-constants
+| pi                                    -- combinators:     Π
+| sigma                                 --                  Σ
+| sing                                  -- star constants:  𝔰
+| bUnion                                --                  ∪ (binary union)
+| iUnion                                --                  ∪ (indexed union)
+| var : string → Term                   -- variables
+| app : Term → Term → Term              -- application of terms
+--deriving BEq, DecidableEq, Repr
+
+--namespace Term
+-- Notation for Terms
+--infixl:70 " □ " => app
+--prefix:90 "` " => var
+
+-- (x:string) (var x)
+
+-- NOTATION: Notation for combinators and star constants
+notation "Π₁" => Term.pi
+notation "Σ₁" => Term.sigma
+notation "𝔰₁" => Term.sing
+notation "∪₁" => Term.bUnion
+notation "ind_⋃₁" => Term.iUnion
+notation t₁ "·" t₂ => Term.app t₁ t₂
+--notation "⁅"t₁ t₂"⁆" => Term.app t₁ t₂
+
+open Term
+
+/-
+-- Substitution function for Terms
+def subst : Term → Sym → Term → Term
+| (var x), y, v => if x = y then v else var x
+| pi, _, _ => pi
+| sigma, _, _ => sigma
+| sing, _, _ => sing
+| bUnion, _, _ => bUnion
+| iUnion, _, _ => iUnion
+| (app l m), y, v => app (subst l y v) (subst m y v)
+-/
+
+
+-- Typing the terms of L^{omega}_*   (term type checking)
+inductive TypeChecking : Term → FType → Prop
+| tcLcons (t : LTerm) : TypeChecking (lcons t) G                                                  -- L-constants have type G
+| tcPi {σ τ} : TypeChecking pi (σ ⟶ (τ ⟶ σ))                                                    -- Π_{σ,τ} : σ ⟶ (τ ⟶ σ)
+| tcSigma {σ τ ρ}: TypeChecking sigma ((σ ⟶ (τ ⟶ ρ)) ⟶ ((σ ⟶ τ) ⟶ (σ ⟶ ρ)))                  -- Σ_{σ,τ,ρ} : (σ ⟶ (τ ⟶ ρ)) ⟶ ((σ ⟶ τ) ⟶ (σ ⟶ ρ))
+| tcSing {σ}: TypeChecking sing (σ ⟶ σ⋆)                                                         -- 𝔰_{σ} : σ⋆
+| tcBUnion {σ}: TypeChecking bUnion (σ⋆ ⟶ (σ⋆ ⟶ σ⋆))                                            -- ∪_{σ} : σ⋆ ⟶ (σ⋆ ⟶ σ⋆)
+| tcIUnion {σ τ} : TypeChecking iUnion (σ⋆ ⟶ ((σ ⟶ τ⋆) ⟶ τ⋆))                                   -- ∪_{σ} : σ⋆ ⟶ ((σ ⟶ τ⋆) ⟶ τ⋆)
+| tcVar {x σ}: TypeChecking (var x) σ                                                             -- Variables x : σ
+| tcApp {t₁ t₂ σ τ}: TypeChecking t₁ (σ ⟶ τ) → TypeChecking t₂ σ → TypeChecking (app t₁ t₂) τ    -- If t₁ : (σ ⟶ τ) and t₂ : σ, then t₁t₂ : τ
+
+open TypeChecking
+
+
+-- ------------------
+-- FORMULAS (p.12-14)
+-- ------------------
+
+-- DEFINITION 1.6 (p.11): Atomic formulas of L^{omega}_*
+inductive AtomicFormula
+| lForm : LFormula → AtomicFormula                                  -- Remark 1.9: The atomic formulas of L^{omega}_* include the atomic formulas of L
+| rel : string → List Term → AtomicFormula                          -- R(t₁, ..., tₙ) with R relational symbol of L and t₁,...,tₙ ground terms in L^{omega}_*
+| eq : FType → Term → Term → AtomicFormula                          -- t =σ q
+| mem : FType → Term → Term → AtomicFormula                         -- t ∈σ q
+
+-- Typing the components of the atomic formulas of L^{omega}_* (atomic formulas type checking)
+inductive AtomicTypeChecking : AtomicFormula → Prop
+| tcRel {R l_terms} :                             -- R é relational symbol DE L (falta); l_terms é uma lista de termos
+    (∀ t, t ∈ l_terms → TypeChecking t G) →
+    AtomicTypeChecking (AtomicFormula.rel R l_terms)
+| tcEq {σ t₁ t₂} :
+    TypeChecking t₁ σ →
+    TypeChecking t₂ σ →
+    AtomicTypeChecking (AtomicFormula.eq σ t₁ t₂)
+| tcMem {σ t₁ t₂} :
+    TypeChecking t₁ σ →
+    TypeChecking t₂ (σ⋆) →
+    AtomicTypeChecking (AtomicFormula.mem σ t₁ t₂)
+
+-- NOTATION: Notation for the equality and the membership symbols
+--notation t₁ "=_" t₂ => AtomicFormula.eq t₁ t₂
+--notation t₁ "∈_"σ t₂ => AtomicFormula.mem σ t₁ t₂
+
+open AtomicFormula
+
+-- DEFINITION 1.10 (p.14): Base formulas of L^{omega}_*
+inductive BaseFormula
+| batom : AtomicFormula → BaseFormula                                   -- Atomic formulas are base formulas
+| bnot : BaseFormula → BaseFormula                                      -- If A is a base formula, then so is (¬A)
+| bor : BaseFormula → BaseFormula → BaseFormula                         -- If A and B are base formulas, then so is (A∨B)
+| bboundedForall : string → FType → Term → BaseFormula → BaseFormula    -- If A is a base formula, then so is (∀x∈t A)
+
+--#check (A : AtomicFormula) batom A
+def SomeFormula (A : AtomicFormula) : BaseFormula := BaseFormula.batom A        -- TESTE
+#check SomeFormula                                                              -- TESTE
+
+-- DEFINITION 1.7 (p.13): Formulas of L^{omega}_*
+inductive Formula
+| Fbase : BaseFormula → Formula                                         -- Base formulas are formulas
+| Fnot : Formula → Formula                                              -- If A is a formula, then so is (¬A)
+| For : Formula → Formula → Formula                                     -- If A and B are formulas, then so is (A∨B)
+| FboundedForall : string → FType → Term → Formula → Formula            -- If A is a formula, then so is (∀x∈t A)
+| FunboundedForall : string → FType → Formula → Formula                 -- If A is a base formula, then so is (∀x A)
+
+-- Type checking for base formulas
+inductive BaseFormulaTypeChecking : BaseFormula → Prop
+| tcBatom {A} :
+    AtomicTypeChecking A → BaseFormulaTypeChecking (BaseFormula.batom A)
+| tcBnot {A} :
+    BaseFormulaTypeChecking A → BaseFormulaTypeChecking (BaseFormula.bnot A)
+| tcBor {A B} :
+    BaseFormulaTypeChecking A →
+    BaseFormulaTypeChecking B →
+    BaseFormulaTypeChecking (BaseFormula.bor A B)
+| tcBboundedForall {x σ t A} :
+    TypeChecking (Term.var x) σ →
+    TypeChecking t (σ⋆) →
+    BaseFormulaTypeChecking A →
+    BaseFormulaTypeChecking (BaseFormula.bboundedForall x σ t A)
+
+-- Type checking for formulas
+inductive FormulaTypeChecking : Formula → Prop
+| tcFbase {A} :
+    BaseFormulaTypeChecking A → FormulaTypeChecking (Formula.Fbase A)
+| tcFnot {A} :
+    FormulaTypeChecking A → FormulaTypeChecking (Formula.Fnot A)
+| tcFor {A B} :
+    FormulaTypeChecking A →
+    FormulaTypeChecking B →
+    FormulaTypeChecking (Formula.For A B)
+| tcFboundedForall {x σ t A} :
+    TypeChecking (Term.var x) σ →
+    TypeChecking t (σ⋆) →
+    FormulaTypeChecking A →
+    FormulaTypeChecking (Formula.FboundedForall x σ t A)
+| tcFunboundedForall {x σ A} :
+    TypeChecking (Term.var x) σ →
+    FormulaTypeChecking A →
+    FormulaTypeChecking (Formula.FunboundedForall x σ A)
+
+-- COPIED UNTIL HERE
+
+open BaseFormula
+open Formula
+
+def AB (A B : Formula) : Formula := Formula.For A B             -- TESTE
+def AB2 (A B : Formula) : Formula := For A B                    -- TESTE
+def ABC (A B C : Formula) : Formula := For A (For B C)          -- TESTE
+
+-- NOTATION: Notation for the primitive symbols ¬, ∨, ∀x and ∀x∈t in L^{omega}_*
+notation "¬₁" A => Fnot A
+notation A "∨₁" B => For A B
+notation "b∀₁" x σ t A => FboundedForall x σ t A
+notation "V₁" x σ A => FunboundedForall x σ A
+
+def ABC2 (A B C : Formula) : Formula := A ∨₁ (B ∨₁ C)           -- TESTE
+def ABC3 (A B C : Formula) : Formula := (A ∨₁ B) ∨₁ C           -- TESTE
+#check ABC2                                                     -- TESTE
+--def ABCABC2 (A B C : Formula) : Formula → Formula := (ABC2 A B C) → (ABC3 A B C)
+--def ABCABC (A B C : Formula) : Formula → Formula := A ∨₁ (B ∨₁ C) → (A ∨₁ B) ∨₁ C
+
+-- --------------------
+-- DEFINED SYMBOLS: Usual logical abbreviations for the defined symbols ∧, →, ↔, ∃x and ∃x∈t in L^{omega}_* (p.8 and p.14)
+-- --------------------
+
+-- Conjunction:  A ∧ B := ¬(¬A∨¬B)
+@[simp]
+def Fand (A B : Formula) : Formula :=
+  ¬₁ ((¬₁ A) ∨₁ (¬₁ B))
+-- have (¬₁ ((¬₁ A) ∨₁ (¬₁ B))) by
+
+-- Implication:  A → B := ¬ A ∨ B
+@[simp]
+def Fimplies (A B : Formula) : Formula :=
+  (¬₁ A) ∨₁ B
+
+notation A "∧₁" B => Fand A B
+notation A "→₁" B => Fimplies A B
+
+-- Equivalence:  A ↔ B := (A → B) ∧ (B → A)
+@[simp]
+def Fiff (A B : Formula) : Formula :=
+  (A →₁ B) ∧₁ (B →₁ A)
+
+-- Existential quantification:  ∃x A := ¬ (∀x (¬ A))
+--def Fexists (x : string) (σ : FType) (A : Formula) : Formula :=
+--  ¬₁(∀₁ "x" σ (¬₁A))
+
+notation A "↔₁" B => Fiff A B
+-- notation "∃₀" x A => exists_L x A
+
+-- ∃x A := ¬ (∀x (¬ A))                                 -- TESTE
+--def lexists (x : LVar) (A : LFormula) : LFormula :=   -- TESTE
+--  ¬₁ (∀₁ x (¬₁ A))                                    -- TESTE
+
+def teste3 (A : Formula) := ¬₁(¬₁ A)                    -- TESTE
+#check teste3                                           -- TESTE
+
+-- --------------------------------------
+-- Notation for the bounded and unbounded universal quantifier
+
+def V (x : string) (σ : FType) (A : Formula) : Formula := FunboundedForall x σ A
+def bV (x : string) (σ : FType) (t : Term) (A : Formula) : Formula := FboundedForall x σ t A
+
+-- --------------------------------------
+
+-- DEFINITION 1.8 (p.14): The bounded existential quantifier ∃x∈t (defined symbol)
+
+-- F_unb_exists
+def E (x : string) (σ : FType) (A : Formula) : Formula :=
+  ¬₁(FunboundedForall x σ (¬₁ A))
+
+-- F_b_exists
+def bE (x : string) (σ : FType) (t : Term) (A : Formula) : Formula :=
+  ¬₁(FboundedForall x σ t (¬₁ A))
+
+-- --------------------
+-- Acrescentar algo que checks whether a formula is base or not
+--  + acrescentar que simbolos definidos também deixam as base formulas closed
+-- --------------------
+
+-- CHECK SE É BASE
+
+def isBase : Formula → Bool
+| Fbase _ => true
+| _ => false
+
+#check isBase
+
+--@[simp]
+def isBaseFormula : Formula → Bool
+| Fbase _ => true
+| ¬₁ (Fbase _) => true
+| (Fbase _) ∨₁ (Fbase _) => true
+| FboundedForall _ _ _ (Formula.Fbase _) => true
+| _ => false
+
+-- Ex1.4(1). tx : τ where t : σ → τ and x : σ                                 -- TESTE
+example (σ τ : FType) (t : Term) (x : string)                                 -- TESTE
+    (h1: TypeChecking t (σ ⟶ τ))                                             -- TESTE
+    (h2 : TypeChecking (var x) σ) : TypeChecking (app t (var x)) τ :=         -- TESTE
+  by                                                                          -- TESTE
+   exact TypeChecking.tcApp h1 h2                                             -- TESTE
+
+lemma teste1 (A : BaseFormula)                                                -- TESTE
+  (hA : isBaseFormula (Fbase A))                                              -- TESTE
+  (hB : isBaseFormula (Fbase B)) : isBaseFormula ((Fbase A) ∨₁ (Fbase B)) :=  -- TESTE
+  by                                                                          -- TESTE
+    simp [isBaseFormula]                                                      -- TESTE
+
+#check teste1                                                                 -- TESTE
+
+
+
+-- Lemma: ¬₁ ((¬₁ A) ∨₁ (¬₁ B)) is a base formula
+--AQUIlemma neg_disjunction_is_base_formula (A B : BaseFormula) (h: bnot (bor (bnot A) (bnot B))) : BaseFormula := sorry
+--begin
+--  exact BaseFormula.bnot (BaseFormula.bor (BaseFormula.bnot A) (BaseFormula.bnot B)),
+--end
+
+--example (A : BaseFormula) (hA : isBaseFormula (Fbase A)) (hB : isBaseFormula (Fbase B)) : isBaseFormula ((¬₁ (Fbase A)) ∨₁ (Fbase B)) :=
+--  by
+--    simp [isBaseFormula]
+  -- by
+  -- exact isBaseFormula
+
+-- lemma (A B : FBase): (A ∧₁ B) : FBase :=
+-- Lemma: if A and B are BaseFormula, then A ∧₁ B is a BaseFormula
+--lemma and_is_baseformula (A B : BaseFormula) : isBaseFormula ((Fbase A) ∧₁ (Fbase B)) = true := sorry
+  ----by
+    -- Acho que devia simplificar usando Fand
+    -----simp
+    -----have h1 := isBaseFormula ((Fbase A) ∨₁ (Fbase B))
+  --by unfold Fand (Fbase A) (Fbase B)
+  --by unfold Fand ; simp [isBaseFormula]
+
+
+
+
+-- ----------------------------------------
+-- EXAMPLE 1.6 (p.14): Base formulas or not
+-- ----------------------------------------
+
+-- example (A : Formula) (B : FBase) (σ τ : FTypes)
+
+
+
+
+
+
+-- --------------------
+-- AXIOMS
+-- --------------------
+
+-- SHOENFIELD'S CALCULUS (Axiom 1.1)
+
+-- -----------------------------------------------------------------------------------
+-- -------------------------- AXIOM SCHEMA -------------------------------------------
+-- -----------------------------------------------------------------------------------
+
+-- Axiom schema:
+
+-- --------------------------- Excluded middle ---------------------------------------
+-- Excluded middle
+
+-- axiom ExcMid (A : Formula) : (¬₁ A) ∨₁ A
+-- axiom ExcMid (A : Formula) : For (Fnot A) A
+
+
+-- Excluded middle DEFINITION
+def excluded_middle_axiom (A : Formula) : Formula :=
+  (¬₁ A) ∨₁ A
+--  For (Fnot A) A
+
+-- Excluded middle AXIOM + AXIOM INSTANCE
+axiom excluded_mid_axiom (A : Formula) : Formula
+axiom excluded_mid_instance (A : Formula) : excluded_middle_axiom A = (¬₁ A) ∨₁ A
+
+-- --------------------------- Substitution (TBDone)---------------------------------
+-- Substituion
+
+-- -----------------------------------------------------------------------------------
+-- --------------------------- RULES -------------------------------------------------
+-- -----------------------------------------------------------------------------------
+
+-- Rules:
+
+-- --------------------------- Expansion ---------------------------------------------
+-- Expansion
+
+def expansion_r (A B : Formula) : Formula :=
+  B ∨₁ A
+
+axiom expansion_rule (A B : Formula) : Formula
+axiom expansion_instance (A B : Formula) : expansion_rule A B = B ∨₁ A
+
+-- --------------------------- Contraction ------------------------------------------
+-- Contraction
+
+def contraction_r (A : Formula) : Formula :=
+  A ∨₁ A
+
+axiom contraction_rule (A : Formula) : Formula
+axiom contraction_instance (A : Formula) : contraction_rule A = A ∨₁ A
+
+-- --------------------------- Associativity ----------------------------------------
+-- Associativity
+
+-- axiom associativity {A B C : Formula} : (A ∨₁ (B ∨₁ C)) → (A ∨₁ B) ∨₁ C
+
+
+--def associativity_r (A B C : Formula) (h : A ∨₁ (B ∨₁ C)) : Formula :=
+--   (A ∨₁ B) ∨₁ C
+
+--def associativity_r (A B C : Formula) (h : (For A (For B C))) : Formula :=
+--   For (For A B) C
+
+--def associativity_r (A B : Formula) : Formula → Formula :=
+--  A → A
+
+--axiom associativity_rule (A B C : Formula) : Formula
+--axiom ass_inst (A B C : Formula) : associativity_rule A B C = (A∨₁(B∨₁C) → (A∨₁B)∨₁C)
+--axiom associativity_instance (A B C : Formula) : (associativity_rule A B C) = A ∨₁ (B ∨₁ C) → (A ∨₁ B) ∨₁ C
+
+--axiom associativity (A B C : Formula) : ((A ∨₁ B) ∨₁ C) → (A ∨₁ (B ∨₁ C))
+
+-- --------------------------- Cut --------------------------------------------------
+-- Cut
+
+-- --------------------------- ∀-introduction ---------------------------------------
+-- ∀-introduction
+
+
+
+
+-- -----------------------------------------------------------------------------------
+-- --------------------------- OTHER AXIOMS -------------------------------------------------
+-- -----------------------------------------------------------------------------------
+
+
+-- EQUALITY AXIOMS (Axiom 1.2)
+
+--axiom equality_reflexivity (σ : FType) (x : var) : Formula :=
+--  ∀₀ x (Term.var x =_σ Term.var x)
+
+
+-- PROPOSITION 1.1: Symmetry and transitivity of equality (higher types)
+
+-- Symmetry of equality   WRONG -> precisamos de TypeChecking?
+--theorem symmetry_of_eq (σ : FType) (x y : string): eq σ (var x) (var y) → eq σ (var y) (var x) := sorry
+-- by intro a intro b exact tcEq hx hy
+-- λ h, h.symm
+
+-- Types in the symmetry of equality   WRONG -> precisamos de TypeChecking?
+--theorem symmetry_of_eq (σ : FType) (x y : string)
+--    (hx : TypeChecking (var x) σ)
+--    (hy : TypeChecking (var y) σ) : (var x) "=_"σ (var y) → (var y) "=_"σ (var x) := sorry
+-- by intro a intro b exact tcEq hx hy
+-- λ h, h.symm
+
+-- #check AtomicFormula.eq σ (var x) (var y)
+
+-- Types in the symmetry of equality   WRONG -> precisamos de TypeChecking?
+--theorem symmetry_of_eq2 (σ : FType) (x y : string)
+--    (hx : TypeChecking (var x) σ)
+--    (hy : TypeChecking (var y) σ)
+--    (hy : TypeChecking (var y) σ): AtomicFormula.eq σ (var x) (var y) → AtomicFormula.eq σ (var y) (var x) := sorry
+-- by intro a intro b exact tcEq hx hy
+-- λ h, h.symm
+
+-- notation t₁ "=_"σ t₂ => AtomicFormula.eq σ t₁ t₂
+
+-- Transitivity of equality   WRONG -> precisamos de TypeChecking?
+-- theorem transitivity_of_eq (σ : FType) (x y z : string) (hx : TypeChecking.tcVar x σ) (hy : TypeChecking.tcVar y σ) (hz : TypeChecking.tcVar z σ) : (var x) "=_"σ (var y) → (var y) "=_"σ (var z) → (var x) "=_"σ (var z) :=
+-- λ hxy hyz, hxy.trans hyz
+
+
+lemma example_lemma (P Q : Prop) (h : P → Q) (p : P) : Q :=
+  h p
+
+-- notation t₁ "=_" t₂ σ => AtomicFormula.eq t₁ t₂ σ
+
+--lemma example_lemma2 (t₁ t₂ : Term) (σ : FType) : (AtomicFormula.eq t₁ t₂ σ) → (AtomicFormula.eq t₁ t₂ σ) := sorry
+
+-- inductive AtomicFormula2
+-- | atrel : string → List Term → AtomicFormula2  -- R(t₁, ..., tₙ)
+-- | ateq : Term → Term → FType → AtomicFormula2  -- t =σ q
+-- | atmem : FType → Term → Term → AtomicFormula2 -- t ∈σ q
+
+-- lemma example_lemma2 (t₁ t₂ : Term) (σ : FType) (h: t₁ "=_" t₂ σ) : (t₁ "=_" t₂ σ) := sorry
+--  intro h
+--  exact h
+
+-- ----------------------------------------------------------------------------------------------------------
+-- ----------------------------------------------------------------------------------------------------------
+
+-- -----------------AXIOM FOR THE BOUNDED UNIVERSAL QUANTIFIER (Axiom 1.3) -----------------
+
+def AxU (σ : FType) (x t : Term) (A : Formula) : Formula            -- FALTA A(x)
+  := (bV x σ t A) ↔₁ (V x σ ((Fbase (batom (mem σ x t))) →₁ A))
+
+-- ----------------------------- COMBINATOR AXIOMS (Axiom 1.4) -----------------------------
+
+def AxC₁ (σ : FType) (p q : Term) : AtomicFormula       -- FALTA TYPECHECKING -> TBDONE AS LEMMA
+  := eq σ ((Π₁·p)·q) q
+
+-- (h: typechecks pri,eirq tqu qnd  )
+def AxC₂ (τ : FType) (p q t : Term) : AtomicFormula     -- FALTA TYPECHECKING
+  := eq τ (((Σ₁·p)·q)·t) ((p·t)·(q·t))
+
+
+-- ---------------- PRIMARY AXIOMS FOR THE STAR CONSTANTS (Axiom 1.5) ----------------------
+
+def AxP₁ (τ : FType) (x y : Term) : AtomicFormula
+  := eq (τ⋆) ((ind_⋃₁·(𝔰₁·x))·y) (x·y)
+
+def AxP₂_atom (τ : FType) (x y z : Term) : AtomicFormula
+  := eq (τ⋆) ((ind_⋃₁·((∪₁·x)·y))·z) ((∪₁·((ind_⋃₁·x)·z))·((ind_⋃₁·y)·z))
+
+def AxP₂_base (τ : FType) (x y z : Term) : BaseFormula
+  := batom (eq (τ⋆) ((ind_⋃₁·((∪₁·x)·y))·z) ((∪₁·((ind_⋃₁·x)·z))·((ind_⋃₁·y)·z)))
+
+def AxP₂_formula (τ : FType) (x y z : Term) : Formula
+  := Fbase (batom (eq (τ⋆) ((ind_⋃₁·((∪₁·x)·y))·z) ((∪₁·((ind_⋃₁·x)·z))·((ind_⋃₁·y)·z))))
+
+-- -------------- SECONDARY AXIOMS FOR THE STAR CONSTANTS (Axiom 1.6) ----------------------
+
+def AxS₁ (σ : FType) (x y : Term) : Formula
+  := Fbase (batom (mem σ x (𝔰₁·y))) ↔₁ Fbase (batom (eq σ x y))
+
+--def AxS₁_ab (σ : FType) (x y : Term) : Formula                  -- ABBREVIATION NOT WORKING
+--  := Fbase (batom (x ∈_ σ (𝔰₁·y))) ↔₁ Fbase (batom (x ∈_ σ y))
+
+def AxS₂ (σ : FType) (x a b: Term) : Formula
+  := Fbase (batom ( mem σ x ((∪₁·a)·b) )) ↔₁  ( ( Fbase ((batom (mem σ x a))) ∨₁ Fbase ((batom (mem σ x b)) )))
+
+def AxS₃ (σ : FType) (x a b f : Term) : Formula
+  := (Fbase (batom (mem σ b ((ind_⋃₁·a)·f)))) ↔₁ (bE x σ a (Fbase (batom ((mem σ b (f·x))))))
+
+-- ---------------------- BOUNDED AXIOM OF CHOICE (Axiom 1.7) -----------------------------
+
+-- This está meh!! f não tem de ser variável...
+def bAC  (x y f : string) (σ : FType) (A : Formula) : Formula        -- FALTA: restricted to base formulas | (x y : var) | tirar tipos
+  := (V x σ (E y σ A)) →₁ (E f σ (V x σ (bE y σ ((var f)·(var x)) A)))
+
+
+-- SUBSTITUIÇAO
+
+-- Pattermatching com "lambda por casos"  FAZER PARA OS OUTROS TERMOS
+--@[simp]
+--def subst (x : string) (p : Term) : Term → Term
+--| (var y) => if x=y then p else var y           -- var substitui logo
+--| (app e1 e2) => app (subst x p e1) (subst x p e2)
+--| x => x                  -- outra coisa qualquer
+
+
+/-
+
+def subst (x : string) (y : Sym) (v l m : Term) : Term → Sym → Term → Term
+| (var x), y, v => if x = y then v else (var x)
+| pi, _, _ => pi
+| sigma, _, _ => sigma
+| sing, _, _ => sing
+| bUnion, _, _ => bUnion
+| iUnion, _, _ => iUnion
+| (app l m), y, v => app (subst l y v) (subst m y v)
+
+-/
+
+
+-- CONVERSIONS
+
+-- Primeira conversion
+def pi_app_transform : Term → Term
+| (Π₁·q)·_ => q
+| t => t
+
+-- Example usage
+--#eval pi_app_transform p
+
+-- Transformation function?
+def pi_app_transform2 : Term → Term
+| (Π₁·q)·_ => q   -- Transforma (Π₁·q)·_ em q
+| t => t             -- Outros casos ficam
+
+-- def pi_app_transform2 : Term → Term → Term
+-- | p q => q
+-- | t => t
+
+def example_term (q t : Term) : Term := (Π₁·q)·t
+#check example_term
+
+
+
+
+end StarLang_old
